code/hash/Hacl.Hash.Definitions.fst
@@ -54,8 +54,8 @@ inline_for_extraction noextract
 let impl_word (i:impl) =
   [@inline_let] let a = get_alg i in
   match a with
+  | SHA2_224 | SHA2_256 | SHA2_384 | SHA2_512
   | MD5 | SHA1 | SHA3_256 -> word a
-  | SHA2_224 | SHA2_256 | SHA2_384 | SHA2_512 -> Hacl.Spec.SHA2.Vec.(element_t a M32)
   | Blake2S | Blake2B -> Blake2.element_t (to_blake_alg a) (get_spec i)
 
 inline_for_extraction noextract
@@ -90,9 +90,8 @@ inline_for_extraction noextract
 let as_seq (#i:impl) (h:HS.mem) (s:state i) : GTot (words_state (get_alg i)) =
   let a = get_alg i in
   match a with
+  | SHA2_224 | SHA2_256 | SHA2_384 | SHA2_512
   | MD5 | SHA1 | SHA3_256 -> B.as_seq h s
-  | SHA2_224 | SHA2_256 | SHA2_384 | SHA2_512 ->
-      Seq.index Hacl.Spec.SHA2.Vec.(state_spec_v #a #M32 (B.as_seq h s)) 0
   | Blake2S -> Blake2.state_v #Spec.Blake2.Blake2S #(get_spec i) h s
   | Blake2B -> Blake2.state_v #Spec.Blake2.Blake2B #(get_spec i) h s
 
